examples/programs/dijkstra/dijkstra_DijkstraShortestPath_WP_parameter_shortest_path_code_2.v
@@ -3,6 +3,7 @@
 Require Import BuiltIn.
 Require BuiltIn.
 Require int.Int.
+Require map.Map.
 
 (* Why3 assumption *)
 Definition unit  := unit.
@@ -117,31 +118,6 @@ Axiom cardinal_subset : forall {a:Type} {a_WT:WhyType a}, forall (s1:(set a))
 Axiom cardinal1 : forall {a:Type} {a_WT:WhyType a}, forall (s:(set a)),
   ((cardinal s) = 1%Z) -> forall (x:a), (mem x s) -> (x = (choose s)).
 
-Axiom map : forall (a:Type) {a_WT:WhyType a} (b:Type) {b_WT:WhyType b}, Type.
-Parameter map_WhyType : forall (a:Type) {a_WT:WhyType a}
-  (b:Type) {b_WT:WhyType b}, WhyType (map a b).
-Existing Instance map_WhyType.
-
-Parameter get: forall {a:Type} {a_WT:WhyType a} {b:Type} {b_WT:WhyType b},
-  (map a b) -> a -> b.
-
-Parameter set1: forall {a:Type} {a_WT:WhyType a} {b:Type} {b_WT:WhyType b},
-  (map a b) -> a -> b -> (map a b).
-
-Axiom Select_eq : forall {a:Type} {a_WT:WhyType a} {b:Type} {b_WT:WhyType b},
-  forall (m:(map a b)), forall (a1:a) (a2:a), forall (b1:b), (a1 = a2) ->
-  ((get (set1 m a1 b1) a2) = b1).
-
-Axiom Select_neq : forall {a:Type} {a_WT:WhyType a}
-  {b:Type} {b_WT:WhyType b}, forall (m:(map a b)), forall (a1:a) (a2:a),
-  forall (b1:b), (~ (a1 = a2)) -> ((get (set1 m a1 b1) a2) = (get m a2)).
-
-Parameter const: forall {a:Type} {a_WT:WhyType a} {b:Type} {b_WT:WhyType b},
-  b -> (map a b).
-
-Axiom Const : forall {a:Type} {a_WT:WhyType a} {b:Type} {b_WT:WhyType b},
-  forall (b1:b) (a1:a), ((get (const b1:(map a b)) a1) = b1).
-
 Axiom vertex : Type.
 Parameter vertex_WhyType : WhyType vertex.
 Existing Instance vertex_WhyType.
@@ -157,8 +133,9 @@ Parameter weight: vertex -> vertex -> Z.
 Axiom Weight_nonneg : forall (x:vertex) (y:vertex), (0%Z <= (weight x y))%Z.
 
 (* Why3 assumption *)
-Definition min(m:vertex) (q:(set vertex)) (d:(map vertex Z)): Prop := (mem m
-  q) /\ forall (x:vertex), (mem x q) -> ((get d m) <= (get d x))%Z.
+Definition min(m:vertex) (q:(set vertex)) (d:(map.Map.map vertex Z)): Prop :=
+  (mem m q) /\ forall (x:vertex), (mem x q) -> ((map.Map.get d
+  m) <= (map.Map.get d x))%Z.
 
 (* Why3 assumption *)
 Inductive path : vertex -> vertex -> Z -> Prop :=
@@ -195,74 +172,78 @@ Definition inv_src(src:vertex) (s:(set vertex)) (q:(set vertex)): Prop :=
   (mem src s) \/ (mem src q).
 
 (* Why3 assumption *)
-Definition inv(src:vertex) (s:(set vertex)) (q:(set vertex)) (d:(map vertex
-  Z)): Prop := (inv_src src s q) /\ (((get d src) = 0%Z) /\ ((subset s v) /\
-  ((subset q v) /\ ((forall (v1:vertex), (mem v1 q) -> ~ (mem v1 s)) /\
-  ((forall (v1:vertex), (mem v1 s) -> (shortest_path src v1 (get d v1))) /\
-  forall (v1:vertex), (mem v1 q) -> (path src v1 (get d v1))))))).
+Definition inv(src:vertex) (s:(set vertex)) (q:(set vertex)) (d:(map.Map.map
+  vertex Z)): Prop := (inv_src src s q) /\ (((map.Map.get d src) = 0%Z) /\
+  ((subset s v) /\ ((subset q v) /\ ((forall (v1:vertex), (mem v1 q) ->
+  ~ (mem v1 s)) /\ ((forall (v1:vertex), (mem v1 s) -> (shortest_path src v1
+  (map.Map.get d v1))) /\ forall (v1:vertex), (mem v1 q) -> (path src v1
+  (map.Map.get d v1))))))).
 
 (* Why3 assumption *)
-Definition inv_succ(src:vertex) (s:(set vertex)) (q:(set vertex)) (d:(map
-  vertex Z)): Prop := forall (x:vertex), (mem x s) -> forall (y:vertex),
-  (mem y (g_succ x)) -> (((mem y s) \/ (mem y q)) /\ ((get d y) <= ((get d
-  x) + (weight x y))%Z)%Z).
+Definition inv_succ(src:vertex) (s:(set vertex)) (q:(set vertex))
+  (d:(map.Map.map vertex Z)): Prop := forall (x:vertex), (mem x s) ->
+  forall (y:vertex), (mem y (g_succ x)) -> (((mem y s) \/ (mem y q)) /\
+  ((map.Map.get d y) <= ((map.Map.get d x) + (weight x y))%Z)%Z).
 
 (* Why3 assumption *)
-Definition inv_succ2(src:vertex) (s:(set vertex)) (q:(set vertex)) (d:(map
-  vertex Z)) (u:vertex) (su:(set vertex)): Prop := forall (x:vertex), (mem x
-  s) -> forall (y:vertex), (mem y (g_succ x)) -> (((~ (x = u)) \/ ((x = u) /\
-  ~ (mem y su))) -> (((mem y s) \/ (mem y q)) /\ ((get d y) <= ((get d
-  x) + (weight x y))%Z)%Z)).
+Definition inv_succ2(src:vertex) (s:(set vertex)) (q:(set vertex))
+  (d:(map.Map.map vertex Z)) (u:vertex) (su:(set vertex)): Prop :=
+  forall (x:vertex), (mem x s) -> forall (y:vertex), (mem y (g_succ x)) ->
+  (((~ (x = u)) \/ ((x = u) /\ ~ (mem y su))) -> (((mem y s) \/ (mem y q)) /\
+  ((map.Map.get d y) <= ((map.Map.get d x) + (weight x y))%Z)%Z)).
 
-Require Import Why3. Ltac ae := why3 "alt-ergo" timelimit 3.
+Require Import Why3.
+Ltac ae := why3 "alt-ergo" timelimit 3.
 Ltac z := why3 "z3" timelimit 3.
 
 (* Why3 goal *)
 Theorem WP_parameter_shortest_path_code : forall (src:vertex) (dst:vertex),
-  forall (d:(map vertex Z)), ((mem src v) /\ (mem dst v)) -> forall (q:(set
-  vertex)) (d1:(map vertex Z)) (visited:(set vertex)), (((forall (x:vertex),
-  ~ (mem x visited)) /\ (q = (add src (empty :(set vertex))))) /\
-  (d1 = (set1 d src 0%Z))) -> forall (q1:(set vertex)) (d2:(map vertex Z))
-  (visited1:(set vertex)), ((((inv_src src visited1 q1) /\ (((get d2
-  src) = 0%Z) /\ ((subset visited1 v) /\ ((subset q1 v) /\
-  ((forall (v1:vertex), (mem v1 q1) -> ~ (mem v1 visited1)) /\
-  ((forall (v1:vertex), (mem v1 visited1) -> (shortest_path src v1 (get d2
-  v1))) /\ forall (v1:vertex), (mem v1 q1) -> (path src v1 (get d2
-  v1)))))))) /\ forall (x:vertex), (mem x visited1) -> forall (y:vertex),
-  (mem y (g_succ x)) -> (((mem y visited1) \/ (mem y q1)) /\ ((get d2
-  y) <= ((get d2 x) + (weight x y))%Z)%Z)) /\ forall (m:vertex), ((mem m
-  q1) /\ forall (x:vertex), (mem x q1) -> ((get d2 m) <= (get d2 x))%Z) ->
-  forall (x:vertex), forall (dx:Z), (path src x dx) -> ((dx < (get d2
-  m))%Z -> (mem x visited1))) -> forall (o:bool), ((o = true) <->
-  forall (x:vertex), ~ (mem x q1)) -> ((~ (o = true)) ->
-  ((~ forall (x:vertex), ~ (mem x q1)) -> forall (q2:(set vertex)),
-  forall (u:vertex), (((mem u q1) /\ forall (x:vertex), (mem x q1) ->
-  ((get d2 u) <= (get d2 x))%Z) /\ (q2 = (remove u q1))) -> (((path src u
-  (get d2 u)) /\ forall (d':Z), (path src u d') -> ((get d2 u) <= d')%Z) ->
+  forall (d:(map.Map.map vertex Z)), ((mem src v) /\ (mem dst v)) ->
+  forall (q:(set vertex)) (d1:(map.Map.map vertex Z)) (visited:(set vertex)),
+  (((forall (x:vertex), ~ (mem x visited)) /\ (q = (add src (empty :(set
+  vertex))))) /\ (d1 = (map.Map.set d src 0%Z))) -> forall (q1:(set vertex))
+  (d2:(map.Map.map vertex Z)) (visited1:(set vertex)), ((((inv_src src
+  visited1 q1) /\ (((map.Map.get d2 src) = 0%Z) /\ ((subset visited1 v) /\
+  ((subset q1 v) /\ ((forall (v1:vertex), (mem v1 q1) -> ~ (mem v1
+  visited1)) /\ ((forall (v1:vertex), (mem v1 visited1) -> (shortest_path src
+  v1 (map.Map.get d2 v1))) /\ forall (v1:vertex), (mem v1 q1) -> (path src v1
+  (map.Map.get d2 v1)))))))) /\ forall (x:vertex), (mem x visited1) ->
+  forall (y:vertex), (mem y (g_succ x)) -> (((mem y visited1) \/ (mem y
+  q1)) /\ ((map.Map.get d2 y) <= ((map.Map.get d2 x) + (weight x
+  y))%Z)%Z)) /\ forall (m:vertex), ((mem m q1) /\ forall (x:vertex), (mem x
+  q1) -> ((map.Map.get d2 m) <= (map.Map.get d2 x))%Z) -> forall (x:vertex),
+  forall (dx:Z), (path src x dx) -> ((dx < (map.Map.get d2 m))%Z -> (mem x
+  visited1))) -> forall (o:bool), ((o = true) <-> forall (x:vertex), ~ (mem x
+  q1)) -> ((~ (o = true)) -> ((~ forall (x:vertex), ~ (mem x q1)) ->
+  forall (q2:(set vertex)), forall (u:vertex), (((mem u q1) /\
+  forall (x:vertex), (mem x q1) -> ((map.Map.get d2 u) <= (map.Map.get d2
+  x))%Z) /\ (q2 = (remove u q1))) -> (((path src u (map.Map.get d2 u)) /\
+  forall (d':Z), (path src u d') -> ((map.Map.get d2 u) <= d')%Z) ->
   forall (visited2:(set vertex)), (visited2 = (add u visited1)) ->
-  forall (su:(set vertex)) (q3:(set vertex)) (d3:(map vertex Z)),
+  forall (su:(set vertex)) (q3:(set vertex)) (d3:(map.Map.map vertex Z)),
   (((forall (x:vertex), (mem x su) -> (mem x (g_succ u))) /\ ((inv_src src
-  visited2 q3) /\ (((get d3 src) = 0%Z) /\ ((subset visited2 v) /\
+  visited2 q3) /\ (((map.Map.get d3 src) = 0%Z) /\ ((subset visited2 v) /\
   ((subset q3 v) /\ ((forall (v1:vertex), (mem v1 q3) -> ~ (mem v1
   visited2)) /\ ((forall (v1:vertex), (mem v1 visited2) -> (shortest_path src
-  v1 (get d3 v1))) /\ forall (v1:vertex), (mem v1 q3) -> (path src v1 (get d3
-  v1))))))))) /\ forall (x:vertex), (mem x visited2) -> forall (y:vertex),
-  (mem y (g_succ x)) -> (((~ (x = u)) \/ ((x = u) /\ ~ (mem y su))) ->
-  (((mem y visited2) \/ (mem y q3)) /\ ((get d3 y) <= ((get d3 x) + (weight x
-  y))%Z)%Z))) -> forall (result:bool), ((result = true) <->
-  ~ forall (x:vertex), ~ (mem x su)) -> ((result = true) ->
-  ((~ forall (x:vertex), ~ (mem x su)) -> forall (su1:(set vertex)),
-  forall (v1:vertex), ((mem v1 su) /\ (su1 = (remove v1 su))) ->
-  forall (q4:(set vertex)) (d4:(map vertex Z)), (((mem v1 visited2) /\
-  ((q4 = q3) /\ (d4 = d3))) \/ (((mem v1 q4) /\ (((get d4 v1) <= ((get d4
-  u) + (weight u v1))%Z)%Z /\ ((q4 = q3) /\ (d4 = d3)))) \/ (((mem v1 q4) /\
-  ((((get d3 u) + (weight u v1))%Z < (get d3 v1))%Z /\ ((q4 = q3) /\
-  (d4 = (set1 d3 v1 ((get d3 u) + (weight u v1))%Z))))) \/ ((~ (mem v1
-  visited2)) /\ ((~ (mem v1 q3)) /\ ((q4 = (add v1 q3)) /\ (d4 = (set1 d3 v1
-  ((get d3 u) + (weight u v1))%Z)))))))) -> ((((get d4 v1) < ((get d4
-  u) + (weight u v1))%Z)%Z \/ ((get d4 v1) = ((get d4 u) + (weight u
-  v1))%Z)) -> forall (v2:vertex), (mem v2 q4) -> (path src v2 (get d4
-  v2)))))))).
+  v1 (map.Map.get d3 v1))) /\ forall (v1:vertex), (mem v1 q3) -> (path src v1
+  (map.Map.get d3 v1))))))))) /\ forall (x:vertex), (mem x visited2) ->
+  forall (y:vertex), (mem y (g_succ x)) -> (((~ (x = u)) \/ ((x = u) /\
+  ~ (mem y su))) -> (((mem y visited2) \/ (mem y q3)) /\ ((map.Map.get d3
+  y) <= ((map.Map.get d3 x) + (weight x y))%Z)%Z))) -> forall (result:bool),
+  ((result = true) <-> ~ forall (x:vertex), ~ (mem x su)) ->
+  ((result = true) -> ((~ forall (x:vertex), ~ (mem x su)) ->
+  forall (su1:(set vertex)), forall (v1:vertex), ((mem v1 su) /\
+  (su1 = (remove v1 su))) -> forall (q4:(set vertex)) (d4:(map.Map.map vertex
+  Z)), (((mem v1 visited2) /\ ((q4 = q3) /\ (d4 = d3))) \/ (((mem v1 q4) /\
+  (((map.Map.get d4 v1) <= ((map.Map.get d4 u) + (weight u v1))%Z)%Z /\
+  ((q4 = q3) /\ (d4 = d3)))) \/ (((mem v1 q4) /\ ((((map.Map.get d3
+  u) + (weight u v1))%Z < (map.Map.get d3 v1))%Z /\ ((q4 = q3) /\
+  (d4 = (map.Map.set d3 v1 ((map.Map.get d3 u) + (weight u v1))%Z))))) \/
+  ((~ (mem v1 visited2)) /\ ((~ (mem v1 q3)) /\ ((q4 = (add v1 q3)) /\
+  (d4 = (map.Map.set d3 v1 ((map.Map.get d3 u) + (weight u v1))%Z)))))))) ->
+  ((((map.Map.get d4 v1) < ((map.Map.get d4 u) + (weight u v1))%Z)%Z \/
+  ((map.Map.get d4 v1) = ((map.Map.get d4 u) + (weight u v1))%Z)) ->
+  forall (v2:vertex), (mem v2 q4) -> (path src v2 (map.Map.get d4 v2)))))))).
 (*
 intros src dst d (h1,h2) q d1 visited ((h3,h4),h5) q1 d2 visited1
 ((h6,(h7,(h8,(h9,(h10,(h11,h12)))))),h14) o h15 h16 h17 q2 u
@@ -272,18 +253,18 @@ su1 v1 (h37,h38) q4 d4 h39 v2 h40.
 *)
 intuition; try ae.
 
-assert (case: (v2 = v1 \/ v2 <> v1)) by ae. destruct case.
-subst v2 d4; rewrite Select_eq.
+destruct (why_decidable_eq v2 v1) as [case|case].
+subst v2 d4; rewrite Map.Select_eq.
 apply Path_cons.
 z.
- ae.
+ae.
 trivial.
-subst d4; rewrite Select_neq.
+subst d4; rewrite Map.Select_neq.
 ae.
 ae.
 
-assert (case: (v2 = v1 \/ v2 <> v1)) by ae. destruct case.
-subst v2 d4; rewrite Select_eq.
+destruct (why_decidable_eq v2 v1) as [case|case].
+subst v2 d4; rewrite Map.Select_eq.
 apply Path_cons.
 z.
 ae.
