examples/programs/edit_distance/edit_distance_WP_EditDistance_WP_parameter_distance_2.v
@@ -4,6 +4,7 @@ Require Import BuiltIn.
 Require BuiltIn.
 Require int.Int.
 Require int.MinMax.
+Require map.Map.
 
 (* Why3 assumption *)
 Definition unit  := unit.
@@ -155,40 +156,15 @@ Definition contents {a:Type} {a_WT:WhyType a}(v:(ref a)): a :=
   | (mk_ref x) => x
   end.
 
-Axiom map : forall (a:Type) {a_WT:WhyType a} (b:Type) {b_WT:WhyType b}, Type.
-Parameter map_WhyType : forall (a:Type) {a_WT:WhyType a}
-  (b:Type) {b_WT:WhyType b}, WhyType (map a b).
-Existing Instance map_WhyType.
-
-Parameter get: forall {a:Type} {a_WT:WhyType a} {b:Type} {b_WT:WhyType b},
-  (map a b) -> a -> b.
-
-Parameter set: forall {a:Type} {a_WT:WhyType a} {b:Type} {b_WT:WhyType b},
-  (map a b) -> a -> b -> (map a b).
-
-Axiom Select_eq : forall {a:Type} {a_WT:WhyType a} {b:Type} {b_WT:WhyType b},
-  forall (m:(map a b)), forall (a1:a) (a2:a), forall (b1:b), (a1 = a2) ->
-  ((get (set m a1 b1) a2) = b1).
-
-Axiom Select_neq : forall {a:Type} {a_WT:WhyType a}
-  {b:Type} {b_WT:WhyType b}, forall (m:(map a b)), forall (a1:a) (a2:a),
-  forall (b1:b), (~ (a1 = a2)) -> ((get (set m a1 b1) a2) = (get m a2)).
-
-Parameter const: forall {a:Type} {a_WT:WhyType a} {b:Type} {b_WT:WhyType b},
-  b -> (map a b).
-
-Axiom Const : forall {a:Type} {a_WT:WhyType a} {b:Type} {b_WT:WhyType b},
-  forall (b1:b) (a1:a), ((get (const b1:(map a b)) a1) = b1).
-
 (* Why3 assumption *)
 Inductive array (a:Type) {a_WT:WhyType a} :=
-  | mk_array : Z -> (map Z a) -> array a.
+  | mk_array : Z -> (map.Map.map Z a) -> array a.
 Axiom array_WhyType : forall (a:Type) {a_WT:WhyType a}, WhyType (array a).
 Existing Instance array_WhyType.
 Implicit Arguments mk_array [[a] [a_WT]].
 
 (* Why3 assumption *)
-Definition elts {a:Type} {a_WT:WhyType a}(v:(array a)): (map Z a) :=
+Definition elts {a:Type} {a_WT:WhyType a}(v:(array a)): (map.Map.map Z a) :=
   match v with
   | (mk_array x x1) => x1
   end.
@@ -200,16 +176,16 @@ Definition length1 {a:Type} {a_WT:WhyType a}(v:(array a)): Z :=
   end.
 
 (* Why3 assumption *)
-Definition get1 {a:Type} {a_WT:WhyType a}(a1:(array a)) (i:Z): a :=
-  (get (elts a1) i).
+Definition get {a:Type} {a_WT:WhyType a}(a1:(array a)) (i:Z): a :=
+  (map.Map.get (elts a1) i).
 
 (* Why3 assumption *)
-Definition set1 {a:Type} {a_WT:WhyType a}(a1:(array a)) (i:Z) (v:a): (array
-  a) := (mk_array (length1 a1) (set (elts a1) i v)).
+Definition set {a:Type} {a_WT:WhyType a}(a1:(array a)) (i:Z) (v:a): (array
+  a) := (mk_array (length1 a1) (map.Map.set (elts a1) i v)).
 
 (* Why3 assumption *)
 Definition make {a:Type} {a_WT:WhyType a}(n:Z) (v:a): (array a) :=
-  (mk_array n (const v:(map Z a))).
+  (mk_array n (map.Map.const v:(map.Map.map Z a))).
 
 Parameter suffix: (array char) -> Z -> (list char).
 
@@ -217,7 +193,7 @@ Axiom suffix_nil : forall (a:(array char)), ((suffix a
   (length1 a)) = (Nil :(list char))).
 
 Axiom suffix_cons : forall (a:(array char)) (i:Z), ((0%Z <= i)%Z /\
-  (i < (length1 a))%Z) -> ((suffix a i) = (Cons (get1 a i) (suffix a
+  (i < (length1 a))%Z) -> ((suffix a i) = (Cons (get a i) (suffix a
   (i + 1%Z)%Z))).
 
 Axiom suffix_length : forall (a:(array char)) (i:Z), ((0%Z <= i)%Z /\
@@ -228,30 +204,33 @@ Definition min_suffix(a1:(array char)) (a2:(array char)) (i:Z) (j:Z)
   (n:Z): Prop := (min_dist (suffix a1 i) (suffix a2 j) n).
 
 (* Why3 goal *)
-Theorem WP_parameter_distance : forall (w1:Z) (w2:Z), forall (w21:(map Z
-  char)) (w11:(map Z char)), let w22 := (mk_array w2 w21) in let w12 :=
-  (mk_array w1 w11) in (((0%Z <= w1)%Z /\ (0%Z <= w2)%Z) ->
-  ((0%Z <= (w2 + 1%Z)%Z)%Z -> ((0%Z <= w2)%Z -> forall (t:(map Z Z)),
-  (forall (j:Z), ((0%Z <= j)%Z /\ (j < (w2 + 1%Z)%Z)%Z) -> ((get t
-  j) = (w2 - j)%Z)) -> ((0%Z <= (w1 - 1%Z)%Z)%Z -> forall (t1:(map Z Z)),
-  forall (i:Z), ((i <= (w1 - 1%Z)%Z)%Z /\ (0%Z <= i)%Z) -> ((forall (j:Z),
-  ((0%Z <= j)%Z /\ (j <= w2)%Z) -> (min_dist (suffix w12 (i + 1%Z)%Z)
-  (suffix w22 j) (get t1 j))) -> (((0%Z <= w2)%Z /\ (w2 < (w2 + 1%Z)%Z)%Z) ->
+Theorem WP_parameter_distance : forall (w1:Z) (w2:Z),
+  forall (w21:(map.Map.map Z char)) (w11:(map.Map.map Z char)), let w22 :=
+  (mk_array w2 w21) in let w12 := (mk_array w1 w11) in (((0%Z <= w1)%Z /\
+  (0%Z <= w2)%Z) -> ((0%Z <= (w2 + 1%Z)%Z)%Z -> ((0%Z <= w2)%Z ->
+  forall (t:(map.Map.map Z Z)), (forall (j:Z), ((0%Z <= j)%Z /\
+  (j < (w2 + 1%Z)%Z)%Z) -> ((map.Map.get t j) = (w2 - j)%Z)) ->
+  ((0%Z <= (w1 - 1%Z)%Z)%Z -> forall (t1:(map.Map.map Z Z)), forall (i:Z),
+  ((i <= (w1 - 1%Z)%Z)%Z /\ (0%Z <= i)%Z) -> ((forall (j:Z), ((0%Z <= j)%Z /\
+  (j <= w2)%Z) -> (min_dist (suffix w12 (i + 1%Z)%Z) (suffix w22 j)
+  (map.Map.get t1 j))) -> (((0%Z <= w2)%Z /\ (w2 < (w2 + 1%Z)%Z)%Z) ->
   (((0%Z <= w2)%Z /\ (w2 < (w2 + 1%Z)%Z)%Z) -> (((0%Z <= w2)%Z /\
-  (w2 < (w2 + 1%Z)%Z)%Z) -> forall (t2:(map Z Z)), (t2 = (set t1 w2 ((get t1
-  w2) + 1%Z)%Z)) -> ((0%Z <= (w2 - 1%Z)%Z)%Z -> forall (oldt:Z) (t3:(map Z
-  Z)), forall (j:Z), ((j <= (w2 - 1%Z)%Z)%Z /\ (0%Z <= j)%Z) ->
-  ((((forall (k:Z), ((j < k)%Z /\ (k <= w2)%Z) -> (min_dist (suffix w12 i)
-  (suffix w22 k) (get t3 k))) /\ forall (k:Z), ((0%Z <= k)%Z /\
-  (k <= j)%Z) -> (min_dist (suffix w12 (i + 1%Z)%Z) (suffix w22 k) (get t3
-  k))) /\ (min_dist (suffix w12 (i + 1%Z)%Z) (suffix w22 (j + 1%Z)%Z)
-  oldt)) -> (((0%Z <= j)%Z /\ (j < (w2 + 1%Z)%Z)%Z) -> forall (oldt1:Z),
-  (oldt1 = (get t3 j)) -> (((0%Z <= j)%Z /\ (j < w2)%Z) -> (((0%Z <= i)%Z /\
-  (i < w1)%Z) -> (((get w11 i) = (get w21 j)) -> (((0%Z <= j)%Z /\
-  (j < (w2 + 1%Z)%Z)%Z) -> forall (t4:(map Z Z)), (t4 = (set t3 j oldt)) ->
-  forall (k:Z), (((j - 1%Z)%Z < k)%Z /\ (k <= w2)%Z) -> (min_dist (suffix w12
-  i) (suffix w22 k) (get t4 k))))))))))))))))).
-(* YOU MAY EDIT THE PROOF BELOW *)
+  (w2 < (w2 + 1%Z)%Z)%Z) -> forall (t2:(map.Map.map Z Z)),
+  (t2 = (map.Map.set t1 w2 ((map.Map.get t1 w2) + 1%Z)%Z)) ->
+  ((0%Z <= (w2 - 1%Z)%Z)%Z -> forall (oldt:Z) (t3:(map.Map.map Z Z)),
+  forall (j:Z), ((j <= (w2 - 1%Z)%Z)%Z /\ (0%Z <= j)%Z) -> ((((forall (k:Z),
+  ((j < k)%Z /\ (k <= w2)%Z) -> (min_dist (suffix w12 i) (suffix w22 k)
+  (map.Map.get t3 k))) /\ forall (k:Z), ((0%Z <= k)%Z /\ (k <= j)%Z) ->
+  (min_dist (suffix w12 (i + 1%Z)%Z) (suffix w22 k) (map.Map.get t3 k))) /\
+  (min_dist (suffix w12 (i + 1%Z)%Z) (suffix w22 (j + 1%Z)%Z) oldt)) ->
+  (((0%Z <= j)%Z /\ (j < (w2 + 1%Z)%Z)%Z) -> forall (oldt1:Z),
+  (oldt1 = (map.Map.get t3 j)) -> (((0%Z <= j)%Z /\ (j < w2)%Z) ->
+  (((0%Z <= i)%Z /\ (i < w1)%Z) -> (((map.Map.get w11 i) = (map.Map.get w21
+  j)) -> (((0%Z <= j)%Z /\ (j < (w2 + 1%Z)%Z)%Z) -> forall (t4:(map.Map.map Z
+  Z)), (t4 = (map.Map.set t3 j oldt)) -> forall (k:Z),
+  (((j - 1%Z)%Z < k)%Z /\ (k <= w2)%Z) -> (min_dist (suffix w12 i)
+  (suffix w22 k) (map.Map.get t4 k))))))))))))))))).
+Proof.
 intuition.
 intuition.
 assert (j=k \/ j < k)%Z by omega. intuition.
@@ -262,14 +241,14 @@ assert (j=k \/ j < k)%Z by omega. intuition.
   rewrite (suffix_cons _ k).
   2: unfold length1; simpl; omega.
   subst.
-  unfold get1; simpl.
-  replace (get w11 i) with (get w21 k).
+  unfold get; simpl.
+  replace (Map.get w11 i) with (Map.get w21 k).
   apply min_dist_equal.
-  rewrite Select_eq; auto.
+  rewrite Map.Select_eq; auto.
   (* j<k *)
   subst.
-  rewrite Select_neq; try omega.
-  assert (min_suffix (mk_array w1 w11) (mk_array w2 w21) i k (get t3 k)); auto with *.
+  rewrite Map.Select_neq; try omega.
+  assert (min_suffix (mk_array w1 w11) (mk_array w2 w21) i k (Map.get t3 k)); auto with *.
 unfold min_suffix.
 intuition.
 Qed.
